Weak union over assumption \#1 implies 
$$
R_1 \indep R_2 \given X_1^{(1)}, X_2^{(1)}, Y
$$
So looking at the presented distribution:
\begin{align*}
    p(r_1, r_2 \given x_1^{(1)}, x_2^{(1)}, y) 
        &= p(r_1 \given x_1^{(1)}, x_2^{(1)}, y) p(r_2 \given x_1^{(1)}, x_2^{(1)}, y) ~\because R_1 \indep R_2 \given X_1^{(1)}, X_2^{(1)}, Y\\
        &= p(r_1 \given x_1, x_2^{(1)}, y) p(r_2 \given x_1^{(1)}, x_2, y) ~\because R_i \indep X_i^{(1)} \given Y, X_j^{(i)}\\\\
    p(r_1 \given x_1, x_2^{(1)}, y) 
        &= p(r_1 \given x_1, x_2^{(1)}, y, r_2 = 1) ~\because R_2 \indep R_1 \given X_2^{(1)}, Y\\
        &= p(r_1 \given x_1, x_2, r_2=1, y) ~\because ~\text{def'n of } R_2\,\& X_2^{(1)}\\\\
    \implies
    p(r_1, r_2 \given x_1^{(1)}, x_2^{(1)}, y)
        &= p(r_1 \given x_1, x_2^{(1)}, y) p(r_2 \given x_1^{(1)}, x_2, y)\\
        &= p(r_1 \given x_1, x_2, r_2=1, y) p(r_2 \given x_1, x_2, r_1=1, y)\\
        &= f(p(y, x_1, x_2, r_1, r_2)) ~~~\blacksquare
\end{align*}